cp

steel/Zeta.Steel.ThreadLogMap.fst
@@ -126,14 +126,18 @@ let owns_anchor_only (m:PM.map tid aval) (tid:tid) =
   has_anchor m tid /\
   None? (perm_of m tid)
 
+
+let related_domains (m:PM.map tid (option log)) (m':PM.map tid aval) =
+    forall tid. has_key m' tid <==> Some? (Map.sel m tid)
+
 let global_anchor_pred (x:t) (m:PM.map tid (option log)) (m':PM.map tid aval)
   : prop
-  = forall (tid:tid). {:pattern (Map.sel m tid) \/ has_key m' tid}
-       (has_key m' tid <==> Some? (Map.sel m tid)) /\
+  = related_domains m m' /\
+    (forall (tid:tid). {:pattern (Map.sel m tid) \/ has_key m' tid}
        (has_key m' tid ==>
          owns_anchor_only m' tid /\
          get m' tid == Some?.v (Map.sel m tid) /\
-         anchor_of m' tid == get m' tid)
+         anchor_of m' tid == get m' tid))
 
 let global_anchor (x:t) ([@@@smt_fallback] m:PM.map tid (option log))
   : vprop
@@ -160,33 +164,36 @@ let global_snapshot (x:t) ([@@@smt_fallback] m: PM.map tid log)
                    get m' tid == Map.sel m tid /\
                    no_ownership m' tid))
 
+
 let tids_pts_to_pred (x:t) (frac:perm) (m:PM.map tid (option log)) (with_anchor:bool) (m': PM.map tid aval)
   : prop
-  = forall (tid:tid).{:pattern (Map.sel m tid) \/ (has_key m' tid)}
-           (has_key m' tid ==> Some? (Map.sel m tid)) /\
-           (Some? (Map.sel m tid) ==> has_key m' tid) /\
+  = related_domains m m' /\
+    (forall (tid:tid).{:pattern (Map.sel m tid) \/ (has_key m' tid)}
            (has_key m' tid ==>
              perm_ok m' tid /\
              perm_of m' tid == Some frac /\
              (with_anchor <==> has_anchor m' tid) /\
-             get m' tid == Some?.v (Map.sel m tid))
+             get m' tid == Some?.v (Map.sel m tid)))
 
-let tids_pts_to (x:t) ([@@@smt_fallback] frac:perm) ([@@@smt_fallback] m:PM.map tid (option log))
+let tids_pts_to (x:t)
+                ([@@@smt_fallback] frac:perm)
+                ([@@@smt_fallback] m:PM.map tid (option log))
+                (with_anchor:bool)
   : vprop
   = exists_ (fun m' ->
     G.pts_to x m' `star`
-    pure (tids_pts_to_pred x frac m false m'))
+    pure (tids_pts_to_pred x frac m with_anchor m'))
 
-let intro_tids_pts_to (#o:_) (x:t) (frac:perm) (m:PM.map tid (option log)) (m':PM.map tid aval)
+let intro_tids_pts_to (#o:_) (x:t) (frac:perm) (m:PM.map tid (option log)) (with_anchor:bool) (m':PM.map tid aval)
   : STGhost unit o
        (G.pts_to x m')
-       (fun _ -> tids_pts_to x frac m)
-       (requires tids_pts_to_pred x frac m false m')
+       (fun _ -> tids_pts_to x frac m with_anchor)
+       (requires tids_pts_to_pred x frac m with_anchor m')
        (ensures fun _ -> True)
-  = intro_pure (tids_pts_to_pred x frac m false m');
+  = intro_pure (tids_pts_to_pred x frac m with_anchor m');
     intro_exists m' (fun m' ->
       G.pts_to x m' `star`
-      pure (tids_pts_to_pred x frac m false m'))
+      pure (tids_pts_to_pred x frac m with_anchor m'))
 
 let alloc0 (#o:_) (_:unit)
   : STGhostT t o
@@ -221,7 +228,7 @@ let split_anchor (m:PM.map tid aval)
 let alloc (#o:_) (_:unit)
   : STGhostT t o
              emp
-             (fun t -> tids_pts_to t full_perm (Map.const (Some Seq.empty)) `star`
+             (fun t -> tids_pts_to t full_perm (Map.const (Some Seq.empty)) false `star`
                     global_anchor t (Map.const (Some Seq.empty)))
   = let m = (Map.const (FAP.Owns (FAP.initial_value Seq.empty))) in
     let x = alloc0 () in
@@ -233,11 +240,11 @@ let alloc (#o:_) (_:unit)
     G.share x m m0 m1;
     assert_ (G.pts_to x m0 `star` G.pts_to x m1);
     let mm0 : PM.map tid (option log) = Map.const (Some Seq.empty) in
-    intro_tids_pts_to x full_perm mm0 m0;
+    intro_tids_pts_to x full_perm mm0 false m0;
     intro_global_anchor x mm0 m1;
     //TODO: leave out these rewrites and the tactic crashes with a scoping error
-    rewrite (tids_pts_to _ _ _)
-            (tids_pts_to x full_perm (Map.const (Some Seq.empty)));
+    rewrite (tids_pts_to _ _ _ _)
+            (tids_pts_to x full_perm (Map.const (Some Seq.empty)) false);
     rewrite (global_anchor _ _)
             (global_anchor x (Map.const (Some Seq.empty)));
     x
@@ -252,6 +259,9 @@ let split_perm (x:FAP.avalue anchors {
   = let (Some p, None), v = x in
     (Some (half_perm p), None), v
 
+#restart-solver
+
+#push-options "--query_stats --fuel 0"
 let split_ownership (frac:perm) (m:PM.map tid aval)
   : Lemma
     (requires
@@ -282,16 +292,16 @@ let share_tids_pts_to_lemma (x:t) (f:perm) (m:PM.map tid (option log)) (m':PM.ma
 
 let share_tids_pts_to (#o:_) (#f:perm) (x:t) (m:PM.map tid (option log))
   : STGhostT unit o
-    (tids_pts_to x f m)
-    (fun _ -> tids_pts_to x (half_perm f) m `star` tids_pts_to x (half_perm f) m)
+    (tids_pts_to x f m false)
+    (fun _ -> tids_pts_to x (half_perm f) m false `star` tids_pts_to x (half_perm f) m false)
   = let m' : erased (PM.map tid aval) = elim_exists () in
     elim_pure _;
     split_ownership f m';
     let half_m' = map_map m' (fun _ -> split_perm) in
     G.share x m' half_m' half_m';
     share_tids_pts_to_lemma x f m m';
-    intro_tids_pts_to x (half_perm f) m half_m';
-    intro_tids_pts_to x (half_perm f) m half_m'
+    intro_tids_pts_to x (half_perm f) m _ half_m';
+    intro_tids_pts_to x (half_perm f) m _ half_m'
 
 let repr_map = PM.map tid (option log)
 
@@ -312,51 +322,28 @@ let take_tid_lemma (x:t) (f:perm) (m:PM.map tid (option log)) (m':PM.map tid ava
       PM.compose_maps fap m0' m1' `Map.equal` m' /\
       tids_pts_to_pred x f (Map.upd m t None) false m0' /\
       tids_pts_to_pred x f (singleton t (Some?.v (Map.sel m t))) false m1'))
-  =  let v = Map.sel m' t in
-     let m0' = Map.upd m' t FAP.Nothing in
-     let m1' = Map.upd (Map.const FAP.Nothing) t v in
-     assert (PM.composable_maps fap m0' m1');
-     assert (PM.compose_maps fap m0' m1' `Map.equal` m');
-     let m' : repr_map = Map.upd m t None in
-     introduce forall (tid:tid).
-           (has_key m0' tid <==> Some? (Map.sel m' tid)) /\
-           (has_key m0' tid ==>
-             perm_ok m0' tid /\
-             perm_of m0' tid == Some f /\
-             ~(has_anchor m0' tid) /\
-             get m0' tid == Some?.v (Map.sel m' tid))
-     with introduce _ /\ _
-     with (())
-     and (());
-     assert (tids_pts_to_pred x f (Map.upd m t None) false m0')
+  =  ()
 
-let tid_pts_to (x:t) (t:tid) ([@@@smt_fallback] frac:perm) ([@@@smt_fallback] l:log)
+let tid_pts_to (x:t) (t:tid) ([@@@smt_fallback] frac:perm) ([@@@smt_fallback] l:log) (with_anchor:bool)
   : vprop
-  = tids_pts_to x frac (singleton t l)
+  = tids_pts_to x frac (singleton t l) with_anchor
 
 let take_tid (#o:_) (#f:perm) (x:t) (m:PM.map tid (option log)) (t:tid { Some? (Map.sel m t) })
   : STGhostT unit o
-    (tids_pts_to x f m)
-    (fun _ -> tid_pts_to x t f (Some?.v (Map.sel m t)) `star`
-           tids_pts_to x f (Map.upd m t None))
+    (tids_pts_to x f m false)
+    (fun _ -> tid_pts_to x t f (Some?.v (Map.sel m t)) false `star`
+           tids_pts_to x f (Map.upd m t None) false)
   = let m' : erased (PM.map tid aval) = elim_exists() in
     elim_pure _;
     take_tid_lemma x f m m' t;
     let m0' = Map.upd m' t FAP.Nothing in
     let m1' = Map.upd (Map.const FAP.Nothing) t (Map.sel m' t) in
     G.share x m' m0' m1';
-    intro_tids_pts_to x f (Map.upd m t None) m0';
+    intro_tids_pts_to x f (Map.upd m t None) false m0';
     let m1 : PM.map tid (option log) = singleton t (Some?.v (Map.sel m t)) in
-    intro_tids_pts_to x f m1 m1';
-    rewrite (tids_pts_to x f m1)
-            (tid_pts_to x t f (Some?.v (Map.sel m t)))
-
-
-let tid_pts_to_with_anchor (x:t) (t:tid) ([@@@smt_fallback] frac:perm) ([@@@smt_fallback] l:log)
-  : vprop
-  = exists_ (fun m' ->
-    G.pts_to x m' `star`
-    pure (tids_pts_to_pred x frac (singleton t l) true m'))
+    intro_tids_pts_to x f m1 false m1';
+    rewrite (tids_pts_to x f m1 false)
+            (tid_pts_to x t f (Some?.v (Map.sel m t)) false)
 
 let take_anchor_tid_lemma (x:t)
                           (m0 m1:PM.map tid aval)
@@ -381,42 +368,17 @@ let take_anchor_tid_lemma (x:t)
       tids_pts_to_pred x f (singleton t l) true m0' /\
       global_anchor_pred x (Map.upd m t None) m1' /\
       PM.composable_maps fap m0' m1' /\
+      PM.compose_maps fap m0' m1' `Map.equal`
+      PM.compose_maps fap m0 m1 /\
       M.committed_log_entries l == Some?.v (Map.sel m t))))
-  = assert (has_key m0 t /\ has_key m1 t);
-    let FAP.Owns ((_, Some anchor), _) = Map.sel m1 t in
-    let FAP.Owns (_, v) = Map.sel m0 t in
-    let av' = (Some f, Some anchor), v in
-    let m0' = Map.upd m0 t (FAP.Owns av') in
-    let m1' = Map.upd m1 t FAP.Nothing in
-    assert (PM.composable_maps fap m0' m1');
-    introduce forall (tid:tid).
-           (has_key m0' tid <==> Some? (Map.sel (singleton t l) tid)) /\ True
-           // (has_key m0' tid ==>
-           //   perm_ok m0' tid /\
-           //   perm_of m0' tid == Some f /\
-           //   (has_anchor m0' tid) /\
-           //   get m0' tid == Some?.v (Map.sel (singleton t l) tid))
-    with introduce _ /\ _
-    with (())
-    and (());
-    assert (tids_pts_to_pred x f (singleton t l) true m0');
-    introduce forall (tid:tid).
-       (has_key m1' tid <==> Some? (Map.sel (Map.upd m t None) tid)) /\ True
-       // (has_key m1' tid ==>
-       //   owns_anchor_only m1' tid /\
-       //   get m1' tid == Some?.v (Map.sel (Map.upd m t None) tid) /\
-       //   anchor_of m1' tid == get m1' tid)
-    with introduce _ /\ _
-    with (())
-    and (());
-    assert (global_anchor_pred x (Map.upd m t None) m1')
+  = ()
 
-let elim_tids_pts_to (#o:_) (x:t) (frac:perm) (m:PM.map tid (option log))
+let elim_tids_pts_to (#o:_) (x:t) (frac:perm) (m:PM.map tid (option log)) (with_anchor:bool)
   : STGhost (erased (PM.map tid aval)) o
-       (tids_pts_to x frac m)
+       (tids_pts_to x frac m with_anchor)
        (fun m' -> G.pts_to x m')
        (requires True)
-       (ensures fun m' -> tids_pts_to_pred x frac m false m')
+       (ensures fun m' -> tids_pts_to_pred x frac m with_anchor m')
   = let m' = elim_exists () in
     elim_pure _;
     m'
@@ -440,18 +402,31 @@ let gpts_to_composable (#o:_) (x:t) (m0 m1:PM.map tid aval)
  = let _ = G.gather x m0 m1 in
    G.share x _ m0 m1
 
+let re_share (#o:_) (x:t) (m0 m1:PM.map tid aval)
+                          (m0' m1':PM.map tid aval)
+  : STGhost unit o
+    (G.pts_to x m0 `star` G.pts_to x m1)
+    (fun _ -> G.pts_to x m0' `star` G.pts_to x m1')
+    (requires
+      PM.composable_maps fap m0 m1 /\
+      PM.composable_maps fap m0' m1' /\
+      PM.compose_maps fap m0' m1' `Map.equal` PM.compose_maps fap m0 m1)
+    (ensures fun _ -> True)
+ = let _ = G.gather x m0 m1 in
+   G.share x _ m0' m1'
+
 let take_anchor_tid (#o:_) (x:t) (m:PM.map tid (option log))
                            (t:tid) (f:perm) (l:log)
   : STGhost unit o
-    (tid_pts_to x t f l `star` global_anchor x m)
-    (fun _ -> tid_pts_to_with_anchor x t f l `star`
+    (tid_pts_to x t f l false `star` global_anchor x m)
+    (fun _ -> tid_pts_to x t f l true `star`
            global_anchor x (Map.upd m t None))
     (requires
       Some? (Map.sel m t))
     (ensures fun _ ->
       Some? (Map.sel m t) /\
       M.committed_log_entries l == Some?.v (Map.sel m t))
-  = let m0 = elim_tids_pts_to x f _ in
+  = let m0 = elim_tids_pts_to x f _ _ in
     let m1 = elim_global_anchor x m in
     gpts_to_composable x m0 m1;
     take_anchor_tid_lemma x m0 m1 m t f l;
@@ -460,13 +435,86 @@ let take_anchor_tid (#o:_) (x:t) (m:PM.map tid (option log))
     let av' = (Some f, Some anchor), v in
     let m0' = Map.upd m0 t (FAP.Owns av') in
     let m1' = Map.upd m1 t FAP.Nothing in
-    admit_()
-    // intro_tids_pts_to x f
-    //   tids_pts_to_pred x f (singleton t l) true m0' /\
-    //   global_anchor_pred x (Map.upd m t None) m1' /\
-    //   PM.composable_maps fap m0' m1' /\
-    //   M.committed_log_entries l == Some?.v (Map.sel m t)
-    // admit_()
+    re_share x m0 m1 m0' m1';
+    intro_tids_pts_to x f (singleton t l) true m0';
+    intro_global_anchor x (Map.upd m t None) m1'
+
+let put_anchor_tid_lemma (x:t)
+                         (m0 m1:PM.map tid aval)
+                         (m:PM.map tid (option log))
+                         (t:tid)
+                         (f:perm)
+                         (l:log)
+  : Lemma
+    (requires
+      tids_pts_to_pred x f (singleton t l) true m0 /\
+      global_anchor_pred x m m1 /\
+      PM.composable_maps fap m0 m1 /\
+      l == M.committed_log_entries l)
+    (ensures (
+      None? (Map.sel m t) /\
+      has_key m0 t /\ (
+      let FAP.Owns av = Map.sel m0 t in
+      let av0, av1 = FAP.anchored_snapshot av in
+      let m0' = Map.upd m0 t (FAP.Owns av0) in
+      let m1' = Map.upd m1 t (FAP.Owns av1) in
+      tids_pts_to_pred x f (singleton t l) false m0' /\
+      global_anchor_pred x (Map.upd m t (Some l)) m1' /\
+      PM.composable_maps fap m0' m1' /\
+      PM.compose_maps fap m0' m1' `Map.equal`
+      PM.compose_maps fap m0 m1)))
+  = ()
+
+let put_anchor_tid (#o:_) (x:t) (m:PM.map tid (option log))
+                          (t:tid) (f:perm) (l:log)
+  : STGhost unit o
+    (tid_pts_to x t f l true `star` global_anchor x m)
+    (fun _ -> tid_pts_to x t f l false `star`
+           global_anchor x (Map.upd m t (Some l)))
+    (requires
+      M.committed_log_entries l == l)
+    (ensures fun _ -> True)
+  = let m0 = elim_tids_pts_to x f _ _ in
+    let m1 = elim_global_anchor x m in
+    gpts_to_composable x m0 m1;
+    put_anchor_tid_lemma x m0 m1 m t f l;
+    let FAP.Owns av = Map.sel m0 t in
+    let av0, av1 = FAP.anchored_snapshot av in
+    let m0' = Map.upd m0 t (FAP.Owns av0) in
+    let m1' = Map.upd m1 t (FAP.Owns av1) in
+    re_share x m0 m1 m0' m1';
+    intro_tids_pts_to x f (singleton t l) false m0';
+    intro_global_anchor x (Map.upd m t (Some l)) m1'
+
+let compat_with_any_anchor_of (l1 l0:log)
+  = forall (anchor:log). anchor `anchors` l0 ==> anchor `anchors` l1
+
+
+let update_tid_log (#o:_) (x:t) (t:tid) (l0 l1:log)
+  : STGhost unit o
+    (tid_pts_to x t full_perm l0 false)
+    (fun _ -> tid_pts_to x t full_perm l1 false)
+    (requires
+      l1 `compat_with_any_anchor_of` l0 /\
+      l0 `log_grows` l1)
+    (ensures fun _ -> True)
+  = let m = elim_tids_pts_to x _ _ _ in
+    G.upd_gen x m _ (update_anchored_value l1 m t);
+    intro_tids_pts_to x full_perm (singleton t l1) false (put_anchored m t l1)
+
+
+let update_anchored_tid_log (#o:_) (x:t) (t:tid) (l0 l1:log)
+  : STGhost unit o
+    (tid_pts_to x t full_perm l0 true)
+    (fun _ -> tid_pts_to x t full_perm l1 true)
+    (requires
+      l0 `log_grows` l1 /\
+      l1 `anchors` l1)
+    (ensures fun _ -> True)
+  = let m = elim_tids_pts_to x _ _ _ in
+    G.upd_gen x m _ (update_value l1 m t);
+    intro_tids_pts_to x full_perm (singleton t l1) true (put m t l1)
+
 
 
 // val global_snapshot (x:t) (m:map tid log)
